Cleanup AtomsAndFacts a bit

ExistentialRules/AtomsAndFacts/Basic.lean
@@ -8,14 +8,12 @@ import ExistentialRules.Terms.ListsOfTerms
 
 section StructuralDefs
 
-  @[ext]
   structure FunctionFreeFact (sig : Signature) [DecidableEq sig.P] [DecidableEq sig.C] where
     predicate : sig.P
     terms : List sig.C
     arity_ok : terms.length = sig.arity predicate
     deriving DecidableEq
 
-  @[ext]
   structure Fact (sig : Signature) [DecidableEq sig.P] [DecidableEq sig.C] [DecidableEq sig.V] where
     predicate : sig.P
     terms : List (GroundTerm sig)
@@ -68,32 +66,24 @@ namespace FunctionFreeAtom
 
   def constants (a : FunctionFreeAtom sig) : List sig.C := VarOrConst.filterConsts a.terms
 
-  def skolemize (ruleId : Nat) (disjunctIndex : Nat) (frontier : List sig.V) (a : FunctionFreeAtom sig) : Atom sig := { predicate := a.predicate, terms := a.terms.map (VarOrConst.skolemize ruleId disjunctIndex frontier), arity_ok := by rw [List.length_map, a.arity_ok] }
+  def skolemize (ruleId : Nat) (disjunctIndex : Nat) (frontier : List sig.V) (a : FunctionFreeAtom sig) : Atom sig := {
+    predicate := a.predicate,
+    terms := a.terms.map (VarOrConst.skolemize ruleId disjunctIndex frontier),
+    arity_ok := by rw [List.length_map, a.arity_ok]
+  }
 
-  theorem skolemize_same_length (ruleId : Nat) (disjunctIndex : Nat) (frontier : List sig.V) (a : FunctionFreeAtom sig) : a.terms.length = (a.skolemize ruleId disjunctIndex frontier).terms.length := by
+  theorem length_skolemize {ruleId : Nat} {disjunctIndex : Nat} {frontier : List sig.V} {a : FunctionFreeAtom sig} :
+      (a.skolemize ruleId disjunctIndex frontier).terms.length = a.terms.length := by
     unfold skolemize
     rw [List.length_map]
 
-  theorem skolem_term_in_skolem_atom_if_term_in_atom (ruleId : Nat) (disjunctIndex : Nat) (frontier : List sig.V) (a : FunctionFreeAtom sig) (t : VarOrConst sig) : t ∈ a.terms.toSet -> (↑(t.skolemize ruleId disjunctIndex frontier)) ∈ (a.skolemize ruleId disjunctIndex frontier).terms.toSet := by
+  theorem mem_skolemize_of_mem {ruleId : Nat} {disjunctIndex : Nat} {frontier : List sig.V}
+      {a : FunctionFreeAtom sig} {t : VarOrConst sig} :
+      t ∈ a.terms -> (t.skolemize ruleId disjunctIndex frontier) ∈ (a.skolemize ruleId disjunctIndex frontier).terms := by
+    intro t_mem
     unfold skolemize
-
-    have : ∀ (ts : List (VarOrConst sig)), t ∈ ts -> (t.skolemize ruleId disjunctIndex frontier) ∈ ts.map (VarOrConst.skolemize ruleId disjunctIndex frontier) := by
-      intro ts
-      induction ts with
-      | nil => intros; contradiction
-      | cons head tail ih =>
-        intro h
-        rw [List.mem_cons] at h
-        rw [List.map_cons, List.mem_cons]
-        cases h with
-        | inl hl => apply Or.inl; simp [Set.element] at hl; rw [hl]
-        | inr hr => apply Or.inr; apply ih; apply hr
-
-    intro mem
-    rw [List.mem_toSet] at mem
-    rw [List.mem_toSet]
-    apply this a.terms
-    exact mem
+    rw [List.mem_map]
+    exists t
 
 end FunctionFreeAtom
 
@@ -113,7 +103,7 @@ namespace Rule
     -- NOTE: using ∈ does not really work here because it produces a Prop which can not always be simply cast into Bool
     List.filter (fun v => r.head.any (fun h => v ∈ h.vars)) (FunctionFreeConjunction.vars r.body)
 
-  theorem frontier_var_occurs_in_fact_in_body (r : Rule sig) : ∀ v, v ∈ r.frontier -> ∃ f, f ∈ r.body ∧ (VarOrConst.var v) ∈ f.terms := by
+  theorem frontier_occurs_in_body (r : Rule sig) : ∀ v, v ∈ r.frontier -> ∃ f, f ∈ r.body ∧ (VarOrConst.var v) ∈ f.terms := by
     unfold frontier
     cases r.body with
     | nil => intros; contradiction
@@ -134,7 +124,7 @@ namespace Rule
   def isDatalog (r : Rule sig) : Bool :=
     r.head.all (fun h => h.vars.all (fun v => v ∈ r.body.vars))
 
-  def isDeterministic (r : Rule sig) : Prop := r.head.length = 1
+  def isDeterministic (r : Rule sig) : Bool := r.head.length = 1
 
   def predicates (r : Rule sig) : List sig.P := r.body.predicates ++ (r.head.flatMap FunctionFreeConjunction.predicates)
 
@@ -200,68 +190,62 @@ namespace RuleSet
 
 end RuleSet
 
-def KnowledgeBase.isDeterministic (kb : KnowledgeBase sig) : Prop := kb.rules.isDeterministic
+namespace KnowledgeBase
 
-def Fact.constants (f : Fact sig) : List sig.C := FiniteTree.leavesList (FiniteTreeList.fromList f.terms.unattach)
-def FactSet.constants (fs : FactSet sig) : Set sig.C := fun c => ∃ f, f ∈ fs ∧ c ∈ f.constants
-theorem FactSet.constants_finite_of_finite (fs : FactSet sig) (fin : fs.finite) : fs.constants.finite := by
-  rcases fin with ⟨l, _, l_eq⟩
-  exists (l.flatMap Fact.constants).eraseDupsKeepRight
-  constructor
-  . apply List.nodup_eraseDupsKeepRight
-  . intro c
-    rw [List.mem_eraseDupsKeepRight]
-    rw [List.mem_flatMap]
-    unfold constants
+  def isDeterministic (kb : KnowledgeBase sig) : Prop := kb.rules.isDeterministic
+
+end KnowledgeBase
+
+namespace Fact
+
+  def constants (f : Fact sig) : List sig.C := f.terms.flatMap GroundTerm.constants
+
+  def function_symbols (f : Fact sig) : List (SkolemFS sig) := f.terms.flatMap GroundTerm.functions
+
+  def isFunctionFree (f : Fact sig) : Prop := ∀ t, t ∈ f.terms -> ∃ c, t = GroundTerm.const c
+
+  def toFunctionFreeFact (f : Fact sig) (isFunctionFree : f.isFunctionFree) : FunctionFreeFact sig := {
+    predicate := f.predicate
+    terms := f.terms.attach.map (fun t => t.val.toConst (isFunctionFree t.val t.property))
+    arity_ok := by rw [List.length_map, List.length_attach, f.arity_ok]
+  }
+
+end Fact
+
+namespace FunctionFreeFact
+
+  def toFact (f : FunctionFreeFact sig) : Fact sig := {
+    predicate := f.predicate,
+    terms := f.terms.map GroundTerm.const,
+    arity_ok := by rw [List.length_map, f.arity_ok]
+  }
+
+  theorem toFact_isFunctionFree (f : FunctionFreeFact sig) : f.toFact.isFunctionFree := by
+    intro t t_mem
+    unfold toFact at t_mem
+    simp at t_mem
+    rcases t_mem with ⟨c, _, t_eq⟩
+    exists c
+    rw [t_eq]
+
+  theorem toFunctionFreeFact_after_toFact_is_id (f : FunctionFreeFact sig) : f.toFact.toFunctionFreeFact (f.toFact_isFunctionFree) = f := by
+    unfold toFact
+    unfold Fact.toFunctionFreeFact
+    simp only
+    rw [FunctionFreeFact.mk.injEq]
     constructor
-    . intro h
-      rcases h with ⟨f, f_mem, c_mem⟩
-      rw [l_eq] at f_mem
-      exists f
-    . intro h
-      rcases h with ⟨f, f_mem, c_mem⟩
-      rw [← l_eq] at f_mem
-      exists f
+    . simp
+    . rw [List.map_attach, List.pmap_map]
+      simp [GroundTerm.toConst, GroundTerm.const]
 
-def Fact.isFunctionFree (f : Fact sig) : Prop := ∀ t, t ∈ f.terms -> ∃ c, t = GroundTerm.const c
-def FactSet.isFunctionFree (fs : FactSet sig) : Prop := ∀ f, f ∈ fs -> f.isFunctionFree
-
-def FunctionFreeFact.toFact (f : FunctionFreeFact sig) : Fact sig := {
-  predicate := f.predicate,
-  terms := f.terms.map GroundTerm.const,
-  arity_ok := by rw [List.length_map, f.arity_ok]
-}
-
-theorem FunctionFreeFact.toFact_isFunctionFree (f : FunctionFreeFact sig) : f.toFact.isFunctionFree := by
-  intro t t_mem
-  unfold toFact at t_mem
-  simp at t_mem
-  rcases t_mem with ⟨c, _, t_eq⟩
-  exists c
-  rw [t_eq]
-
-def Fact.toFunctionFreeFact (f : Fact sig) (isFunctionFree : f.isFunctionFree) : FunctionFreeFact sig :={
-  predicate := f.predicate
-  terms := f.terms.attach.map (fun t => t.val.toConst (isFunctionFree t.val t.property))
-  arity_ok := by rw [List.length_map, List.length_attach, f.arity_ok]
-}
-
-theorem FunctionFreeFact.toFunctionFreeFact_after_toFact_is_id (f : FunctionFreeFact sig) : f.toFact.toFunctionFreeFact (f.toFact_isFunctionFree) = f := by
-  unfold toFact
-  unfold Fact.toFunctionFreeFact
-  simp only
-  apply FunctionFreeFact.ext
-  . simp
-  . simp only
-    rw [List.map_attach, List.pmap_map]
-    simp only [GroundTerm.toConst, GroundTerm.const]
-    simp
+end FunctionFreeFact
 
 theorem Fact.toFact_after_toFunctionFreeFact_is_id (f : Fact sig) (isFunctionFree : f.isFunctionFree) : (f.toFunctionFreeFact isFunctionFree).toFact = f := by
   unfold toFunctionFreeFact
   unfold FunctionFreeFact.toFact
   simp
-  apply Fact.ext
+  rw [Fact.mk.injEq]
+  constructor
   . simp
   . simp only [List.map_attach]
     apply List.ext_get
@@ -275,184 +259,209 @@ theorem Fact.toFact_after_toFunctionFreeFact_is_id (f : Fact sig) (isFunctionFre
     unfold GroundTerm.toConst
     simp
 
-def FactSet.terms (fs : FactSet sig) : Set (GroundTerm sig) := fun t => ∃ f, f ∈ fs ∧ t ∈ f.terms
+namespace FactSet
 
-theorem FactSet.terms_finite_of_finite (fs : FactSet sig) (finite : fs.finite) : fs.terms.finite := by
-  rcases finite with ⟨l, nodup, finite⟩
-  exists (l.map Fact.terms).flatten.eraseDupsKeepRight
-  constructor
-  . apply List.nodup_eraseDupsKeepRight
-  . intro e
-    constructor
-    . intro in_l
-      unfold FactSet.terms
-      simp [List.mem_eraseDupsKeepRight, List.mem_flatten] at in_l
-      rcases in_l with ⟨terms, ex_f, e_in_terms⟩
-      rcases ex_f with ⟨f, f_in_l, terms_eq⟩
-      exists f
-      constructor
-      . rw [← finite]; exact f_in_l
-      . rw [terms_eq]; exact e_in_terms
-    . intro in_fs
-      unfold FactSet.terms at in_fs
-      simp [List.mem_eraseDupsKeepRight, List.mem_flatten]
-      rcases in_fs with ⟨f, f_in_fs, e_in_f⟩
-      exists f.terms
-      constructor
-      . exists f
-        constructor
-        . rw [finite]; exact f_in_fs
-        . rfl
-      . exact e_in_f
+  def predicates (fs : FactSet sig) : Set sig.P := fun p => ∃ f, f ∈ fs ∧ f.predicate = p
 
-def FactSet.predicates (fs : FactSet sig) : Set sig.P := fun p => ∃ f, f ∈ fs ∧ f.predicate = p
+  def terms (fs : FactSet sig) : Set (GroundTerm sig) := fun t => ∃ f, f ∈ fs ∧ t ∈ f.terms
 
-def Fact.function_symbols (f : Fact sig) : Set (SkolemFS sig) := fun func => ∃ t, t ∈ f.terms ∧ func ∈ t.val.innerLabels
-def FactSet.function_symbols (fs : FactSet sig) : Set (SkolemFS sig) := fun func => ∃ f, f ∈ fs ∧ func ∈ f.function_symbols
+  def constants (fs : FactSet sig) : Set sig.C := fun c => ∃ f, f ∈ fs ∧ c ∈ f.constants
 
-theorem FactSet.finite_of_preds_finite_of_terms_finite (fs : FactSet sig) : fs.predicates.finite -> fs.terms.finite -> fs.finite := by
-  intro preds_fin terms_fin
-  rcases preds_fin with ⟨preds, _, preds_eq⟩
-  rcases terms_fin with ⟨terms, _, terms_eq⟩
+  def function_symbols (fs : FactSet sig) : Set (SkolemFS sig) := fun func => ∃ f, f ∈ fs ∧ func ∈ f.function_symbols
 
-  let overapproximation : FactSet sig := fun f => f.predicate ∈ fs.predicates ∧ (∀ t, t ∈ f.terms -> t ∈ fs.terms)
-  have overapproximation_fin : overapproximation.finite := by
-    exists (preds.flatMap (fun p =>
-      (all_term_lists_of_length terms (sig.arity p)).attach.map (fun ⟨ts, mem⟩ =>
-        {
-          predicate := p
-          terms := ts
-          arity_ok := ((mem_all_term_lists_of_length terms (sig.arity p) ts).mp mem).left
-        }
-      )
-    )).eraseDupsKeepRight
+  def isFunctionFree (fs : FactSet sig) : Prop := ∀ f, f ∈ fs -> f.isFunctionFree
 
+  theorem terms_finite_of_finite (fs : FactSet sig) (finite : fs.finite) : fs.terms.finite := by
+    rcases finite with ⟨l, nodup, finite⟩
+    exists (l.map Fact.terms).flatten.eraseDupsKeepRight
     constructor
     . apply List.nodup_eraseDupsKeepRight
-    . intro f
-      rw [List.mem_eraseDupsKeepRight]
-      simp only [List.mem_flatMap, List.mem_map, List.mem_attach, true_and, Subtype.exists]
+    . intro e
       constructor
-      . intro h
-        rcases h with ⟨pred, pred_mem, ts, ts_mem, f_eq⟩
-        rw [← f_eq]
+      . intro in_l
+        unfold FactSet.terms
+        simp [List.mem_eraseDupsKeepRight, List.mem_flatten] at in_l
+        rcases in_l with ⟨terms, ex_f, e_in_terms⟩
+        rcases ex_f with ⟨f, f_in_l, terms_eq⟩
+        exists f
         constructor
-        . rw [preds_eq] at pred_mem
-          exact pred_mem
-        . rw [mem_all_term_lists_of_length] at ts_mem
-          intro t t_mem
-          rw [← terms_eq]
-          apply ts_mem.right
-          exact t_mem
-      . intro h
-        rcases h with ⟨pred_mem, ts_mem⟩
-        exists f.predicate
+        . rw [← finite]; exact f_in_l
+        . rw [terms_eq]; exact e_in_terms
+      . intro in_fs
+        unfold FactSet.terms at in_fs
+        simp [List.mem_eraseDupsKeepRight, List.mem_flatten]
+        rcases in_fs with ⟨f, f_in_fs, e_in_f⟩
+        exists f.terms
         constructor
-        . rw [preds_eq]; exact pred_mem
-        . exists f.terms
-          exists (by
-            rw [mem_all_term_lists_of_length]
-            constructor
-            . exact f.arity_ok
-            . intro t t_mem; rw [terms_eq]; apply ts_mem; exact t_mem
-          )
+        . exists f
+          constructor
+          . rw [finite]; exact f_in_fs
+          . rfl
+        . exact e_in_f
 
-  apply Set.finite_of_subset_finite overapproximation_fin
-  intro f f_mem
-  constructor
-  . exists f
-  . intro t t_mem
-    exists f
-
-def Database.constants (db : Database sig) : { C : Set sig.C // C.finite } := ⟨
-  fun c => ∃ (f : FunctionFreeFact sig), f ∈ db ∧ c ∈ f.terms,
-  by
-    rcases db.property with ⟨l, _, l_eq⟩
-    exists (l.flatMap (fun f => f.terms)).eraseDupsKeepRight
+  theorem constants_finite_of_finite (fs : FactSet sig) (fin : fs.finite) : fs.constants.finite := by
+    rcases fin with ⟨l, _, l_eq⟩
+    exists (l.flatMap Fact.constants).eraseDupsKeepRight
     constructor
     . apply List.nodup_eraseDupsKeepRight
     . intro c
-      rw [List.mem_eraseDupsKeepRight, List.mem_flatMap]
+      rw [List.mem_eraseDupsKeepRight]
+      rw [List.mem_flatMap]
+      unfold constants
       constructor
       . intro h
         rcases h with ⟨f, f_mem, c_mem⟩
+        rw [l_eq] at f_mem
         exists f
-        constructor
-        . rw [l_eq] at f_mem
-          exact f_mem
-        . exact c_mem
       . intro h
         rcases h with ⟨f, f_mem, c_mem⟩
+        rw [← l_eq] at f_mem
         exists f
+
+  theorem finite_of_preds_finite_of_terms_finite (fs : FactSet sig) : fs.predicates.finite -> fs.terms.finite -> fs.finite := by
+    intro preds_fin terms_fin
+    rcases preds_fin with ⟨preds, _, preds_eq⟩
+    rcases terms_fin with ⟨terms, _, terms_eq⟩
+
+    let overapproximation : FactSet sig := fun f => f.predicate ∈ fs.predicates ∧ (∀ t, t ∈ f.terms -> t ∈ fs.terms)
+    have overapproximation_fin : overapproximation.finite := by
+      exists (preds.flatMap (fun p =>
+        (all_term_lists_of_length terms (sig.arity p)).attach.map (fun ⟨ts, mem⟩ =>
+          {
+            predicate := p
+            terms := ts
+            arity_ok := ((mem_all_term_lists_of_length terms (sig.arity p) ts).mp mem).left
+          }
+        )
+      )).eraseDupsKeepRight
+
+      constructor
+      . apply List.nodup_eraseDupsKeepRight
+      . intro f
+        rw [List.mem_eraseDupsKeepRight]
+        simp only [List.mem_flatMap, List.mem_map, List.mem_attach, true_and, Subtype.exists]
         constructor
-        . rw [← l_eq] at f_mem
-          exact f_mem
-        . exact c_mem
-⟩
+        . intro h
+          rcases h with ⟨pred, pred_mem, ts, ts_mem, f_eq⟩
+          rw [← f_eq]
+          constructor
+          . rw [preds_eq] at pred_mem
+            exact pred_mem
+          . rw [mem_all_term_lists_of_length] at ts_mem
+            intro t t_mem
+            rw [← terms_eq]
+            apply ts_mem.right
+            exact t_mem
+        . intro h
+          rcases h with ⟨pred_mem, ts_mem⟩
+          exists f.predicate
+          constructor
+          . rw [preds_eq]; exact pred_mem
+          . exists f.terms
+            exists (by
+              rw [mem_all_term_lists_of_length]
+              constructor
+              . exact f.arity_ok
+              . intro t t_mem; rw [terms_eq]; apply ts_mem; exact t_mem
+            )
 
-def Database.toFactSet (db : Database sig) : { fs : FactSet sig // fs.finite ∧ fs.isFunctionFree } := ⟨
-  (fun f => ∃ f', f' ∈ db.val ∧ f'.toFact = f),
-  (by
-    rcases db.property with ⟨l, _, l_eq⟩
-    exists (l.map FunctionFreeFact.toFact).eraseDupsKeepRight
-    constructor
-    . apply List.nodup_eraseDupsKeepRight
-    . intro f
-      rw [List.mem_eraseDupsKeepRight]
-      rw [List.mem_map]
-      simp only [l_eq]
-      simp [Set.element]
-  ),
-  (by
+    apply Set.finite_of_subset_finite overapproximation_fin
     intro f f_mem
-    rcases f_mem with ⟨_, _, f_eq⟩
-    rw [← f_eq]
-    apply FunctionFreeFact.toFact_isFunctionFree
-  ),
-⟩
-
-theorem Database.toFactSet_constants_same (db : Database sig) : db.toFactSet.val.constants = db.constants.val := by
-  unfold toFactSet
-  unfold constants
-  unfold FactSet.constants
-  simp only
-  apply funext
-  intro c
-  rw [eq_iff_iff]
-  constructor
-  . intro h
-    rcases h with ⟨f, f_mem, c_mem⟩
-    rcases f_mem with ⟨f', f'_mem, f_eq⟩
-    exists f'
-    constructor
-    . exact f'_mem
-    . unfold Fact.constants at c_mem
-      rw [FiniteTree.mem_leavesList] at c_mem
-      rcases c_mem with ⟨t, t_mem, c_mem⟩
-      rw [FiniteTreeList.fromListToListIsId] at t_mem
-      rw [← f_eq] at t_mem
-      unfold FunctionFreeFact.toFact at t_mem
-      unfold List.unattach at t_mem
-      rw [List.map_map, List.mem_map] at t_mem
-      rcases t_mem with ⟨d, d_mem, t_eq⟩
-      rw [← t_eq] at c_mem
-      unfold FiniteTree.leaves at c_mem
-      simp only [Function.comp_apply, GroundTerm.const, List.mem_singleton] at c_mem
-      rw [c_mem]
-      exact d_mem
-  . intro h
-    rcases h with ⟨f, f_mem, c_mem⟩
-    exists f.toFact
     constructor
     . exists f
-    . unfold FunctionFreeFact.toFact
-      unfold Fact.constants
-      rw [FiniteTree.mem_leavesList]
-      exists GroundTerm.const c
+    . intro t t_mem
+      exists f
+
+end FactSet
+
+namespace Database
+
+  def constants (db : Database sig) : { C : Set sig.C // C.finite } := ⟨
+    fun c => ∃ (f : FunctionFreeFact sig), f ∈ db ∧ c ∈ f.terms,
+    by
+      rcases db.property with ⟨l, _, l_eq⟩
+      exists (l.flatMap (fun f => f.terms)).eraseDupsKeepRight
       constructor
-      . rw [FiniteTreeList.fromListToListIsId]
-        unfold List.unattach
-        rw [List.map_map, List.mem_map]
-        exists c
-      . simp [FiniteTree.leaves, GroundTerm.const]
+      . apply List.nodup_eraseDupsKeepRight
+      . intro c
+        rw [List.mem_eraseDupsKeepRight, List.mem_flatMap]
+        constructor
+        . intro h
+          rcases h with ⟨f, f_mem, c_mem⟩
+          exists f
+          constructor
+          . rw [l_eq] at f_mem
+            exact f_mem
+          . exact c_mem
+        . intro h
+          rcases h with ⟨f, f_mem, c_mem⟩
+          exists f
+          constructor
+          . rw [← l_eq] at f_mem
+            exact f_mem
+          . exact c_mem
+  ⟩
+
+  def toFactSet (db : Database sig) : { fs : FactSet sig // fs.finite ∧ fs.isFunctionFree } := ⟨
+    (fun f => ∃ f', f' ∈ db.val ∧ f'.toFact = f),
+    (by
+      rcases db.property with ⟨l, _, l_eq⟩
+      exists (l.map FunctionFreeFact.toFact).eraseDupsKeepRight
+      constructor
+      . apply List.nodup_eraseDupsKeepRight
+      . intro f
+        rw [List.mem_eraseDupsKeepRight]
+        rw [List.mem_map]
+        simp only [l_eq]
+        simp [Set.element]
+    ),
+    (by
+      intro f f_mem
+      rcases f_mem with ⟨_, _, f_eq⟩
+      rw [← f_eq]
+      apply FunctionFreeFact.toFact_isFunctionFree
+    ),
+  ⟩
+
+  theorem toFactSet_constants_same (db : Database sig) : db.toFactSet.val.constants = db.constants.val := by
+    unfold toFactSet
+    unfold constants
+    unfold FactSet.constants
+    simp only
+    apply funext
+    intro c
+    rw [eq_iff_iff]
+    constructor
+    . intro h
+      rcases h with ⟨f, f_mem, c_mem⟩
+      rcases f_mem with ⟨f', f'_mem, f_eq⟩
+      exists f'
+      constructor
+      . exact f'_mem
+      . unfold Fact.constants at c_mem
+        rw [List.mem_flatMap] at c_mem
+        rcases c_mem with ⟨t, t_mem, c_mem⟩
+        rw [← f_eq] at t_mem
+        unfold FunctionFreeFact.toFact at t_mem
+        rw [List.mem_map] at t_mem
+        rcases t_mem with ⟨d, d_mem, t_eq⟩
+        rw [← t_eq] at c_mem
+        rw [GroundTerm.constants_const, List.mem_singleton] at c_mem
+        rw [c_mem]
+        exact d_mem
+    . intro h
+      rcases h with ⟨f, f_mem, c_mem⟩
+      exists f.toFact
+      constructor
+      . exists f
+      . unfold FunctionFreeFact.toFact
+        unfold Fact.constants
+        rw [List.mem_flatMap]
+        exists GroundTerm.const c
+        constructor
+        . rw [List.mem_map]
+          exists c
+        . simp [GroundTerm.constants_const]
+
+end Database
 
