ExistentialRules/AtomsAndFacts/SubstitutionsAndHomomorphisms.lean
@@ -10,9 +10,6 @@ section Defs
 
   abbrev GroundTermMapping := GroundTerm sig -> GroundTerm sig
 
-  class SubsTarget (α) (β) where
-    apply : GroundSubstitution sig -> α -> β
-
 end Defs
 
 namespace GroundSubstitution
@@ -26,22 +23,11 @@ namespace GroundSubstitution
   def apply_skolem_term (σ : GroundSubstitution sig) : SkolemTerm sig -> GroundTerm sig
     | .var v => σ v
     | .const c => GroundTerm.const c
-    | .func fs frontier arity_ok => ⟨
-      FiniteTree.inner fs (FiniteTreeList.fromList (frontier.map (fun fv => σ fv))),
-      by
-        unfold PreGroundTerm.arity_ok
-        rw [Bool.and_eq_true]
-        constructor
-        . rw [FiniteTreeList.fromListToListIsId]
-          rw [List.length_map, beq_iff_eq]
-          exact arity_ok
-        . rw [← PreGroundTerm.arity_ok_list_iff_arity_ok_each_mem]
-          intro t t_mem
-          rw [FiniteTreeList.fromListToListIsId, List.mem_map] at t_mem
-          rcases t_mem with ⟨v, v_mem, t_eq⟩
-          rw [← t_eq]
-          exact (σ v).property
-    ⟩
+    | .func fs frontier arity_ok =>
+      GroundTerm.func fs (frontier.map (fun fv => σ fv)) (by
+        rw [List.length_map]
+        exact arity_ok
+      )
 
   def apply_atom (σ : GroundSubstitution sig) (ϕ : Atom sig) : Fact sig :=
     { predicate := ϕ.predicate, terms := List.map (apply_skolem_term σ) ϕ.terms, arity_ok := by rw [List.length_map, ϕ.arity_ok] }
@@ -52,57 +38,9 @@ namespace GroundSubstitution
   def apply_function_free_conj (σ : GroundSubstitution sig) (conj : FunctionFreeConjunction sig) : List (Fact sig) :=
     (List.map (apply_function_free_atom σ)) conj
 
-  theorem apply_same_length (σ : GroundSubstitution sig) (a : Atom sig) : a.terms.length = (σ.apply_atom a).terms.length := by
+  theorem length_terms_apply_atom (σ : GroundSubstitution sig) (a : Atom sig) :
+      (σ.apply_atom a).terms.length = a.terms.length := by
     simp [apply_atom]
-
-  theorem eq_under_subs_means_same_length (σ : GroundSubstitution sig) (a : Atom sig) (f : Fact sig) (h : σ.apply_atom a = f) : (a.terms.length = f.terms.length) := by
-    rw [← h]
-    simp [apply_atom]
-
-  theorem eq_under_subs_means_term_is_eq (σ : GroundSubstitution sig) (a : Atom sig) (f : Fact sig) (idx : Fin a.terms.length) (h : σ.apply_atom a = f) : (σ.apply_skolem_term (a.terms.get idx) = f.terms.get { val := idx.val, isLt := (by rw [← eq_under_subs_means_same_length σ a f h]; exact idx.isLt) }) := by
-    cases h
-    simp [apply_atom]
-
-  -- TODO: is the extra assumption with injectivity reasonable?
-  theorem eq_under_subs_means_elements_are_preserved (σ : GroundSubstitution sig) (a : Atom sig) (f : Fact sig) (h : σ.apply_atom a = f) : ∀ t, (∀ s, s ∈ a.terms.toSet ∧ σ.apply_skolem_term t = σ.apply_skolem_term s -> t = s) -> ((σ.apply_skolem_term t) ∈ f.terms ↔ t ∈ a.terms) := by
-    intro t ht
-    rw [List.mem_iff_get]
-    rw [List.mem_iff_get]
-    constructor
-    . intro ⟨i, hi⟩
-      let j : Fin a.terms.length := ⟨i.val, (by rw [eq_under_subs_means_same_length σ a f h]; exact i.isLt)⟩
-      exists j
-      rw [← eq_under_subs_means_term_is_eq σ a f j h] at hi
-      apply Eq.symm
-      apply ht
-      constructor
-      . rw [List.get_eq_getElem]
-        apply List.get_mem_toSet
-      . rw [hi]
-    . intro ⟨i, hi⟩
-      let j : Fin f.terms.length := ⟨i.val, (by rw [← eq_under_subs_means_same_length σ a f h]; exact i.isLt)⟩
-      exists j
-      rw [← eq_under_subs_means_term_is_eq σ a f i h]
-      rw [hi]
-
-  -- TODO: is the extra assumption with injectivity reasonable?
-  theorem eq_under_subs_means_indices_of_elements_are_preserved (σ : GroundSubstitution sig) (a : Atom sig) (f : Fact sig) (h : σ.apply_atom a = f) (t : SkolemTerm sig) (ht : t ∈ a.terms) (hs : ∀ s, s ∈ a.terms.toSet ∧ σ.apply_skolem_term t = σ.apply_skolem_term s -> t = s) : (f.terms.idx_of (by rw [eq_under_subs_means_elements_are_preserved σ a f h t hs]; exact ht)).val = (a.terms.idx_of ht).val := by
-    have : f.terms = a.terms.map σ.apply_skolem_term := by rw [← h]; unfold apply_atom; simp
-    rw [List.idx_of_eq_of_list_eq this]
-    apply Eq.symm
-    apply List.idx_of_eq_under_map
-    apply hs
-
-  instance : SubsTarget sig (SkolemTerm sig) (GroundTerm sig) where
-    apply := GroundSubstitution.apply_skolem_term
-  -- instance : SubsTarget Term GroundTerm where
-  --   apply := GroundSubstitution.apply_term
-  instance : SubsTarget sig (Atom sig) (Fact sig) where
-    apply := GroundSubstitution.apply_atom
-  instance : SubsTarget sig (FunctionFreeAtom sig) (Fact sig) where
-    apply := GroundSubstitution.apply_function_free_atom
-  instance : SubsTarget sig (FunctionFreeConjunction sig) (List (Fact sig)) where
-    apply := GroundSubstitution.apply_function_free_conj
 
 end GroundSubstitution
 
@@ -116,12 +54,17 @@ namespace GroundTermMapping
     | .const _ => h t = t
     | _ => True
 
-  theorem apply_constant_is_id_of_isIdOnConstants {h : GroundTermMapping sig} (isId : h.isIdOnConstants) (c : sig.C) : h (GroundTerm.const c) = GroundTerm.const c := isId (GroundTerm.const c)
+  theorem apply_constant_is_id_of_isIdOnConstants {h : GroundTermMapping sig} (isId : h.isIdOnConstants) (c : sig.C) :
+      h (GroundTerm.const c) = GroundTerm.const c :=
+    isId (GroundTerm.const c)
 
   variable [DecidableEq sig.P]
 
-  def applyFact (h : GroundTermMapping sig) (f : Fact sig) : Fact sig :=
-    { predicate := f.predicate, terms := List.map h f.terms, arity_ok := by rw [List.length_map, f.arity_ok] }
+  def applyFact (h : GroundTermMapping sig) (f : Fact sig) : Fact sig := {
+    predicate := f.predicate,
+    terms := List.map h f.terms,
+    arity_ok := by rw [List.length_map, f.arity_ok]
+  }
 
   theorem applyFact_compose (g h : GroundTermMapping sig) : applyFact (h ∘ g) = (applyFact h) ∘ (applyFact g) := by
     apply funext
@@ -152,13 +95,15 @@ namespace GroundTermMapping
       . exact f''_mem
       . rw [f''_eq, f'_eq]
 
-  theorem applyPreservesElement (h : GroundTermMapping sig) (f : Fact sig) (fs : FactSet sig) : f ∈ fs -> applyFact h f ∈ applyFactSet h fs := by
+  theorem applyPreservesElement (h : GroundTermMapping sig) (f : Fact sig) (fs : FactSet sig) :
+      f ∈ fs -> applyFact h f ∈ applyFactSet h fs := by
     intro hf
     simp [Set.element] at *
     unfold applyFactSet
     exists f
 
-  theorem applyFactSet_subset_of_subset (h : GroundTermMapping sig) (as bs : FactSet sig) : as ⊆ bs -> h.applyFactSet as ⊆ h.applyFactSet bs := by
+  theorem applyFactSet_subset_of_subset (h : GroundTermMapping sig) (as bs : FactSet sig) :
+      as ⊆ bs -> h.applyFactSet as ⊆ h.applyFactSet bs := by
     intro subset
     unfold GroundTermMapping.applyFactSet
     intro f f_mem
@@ -202,7 +147,8 @@ section GroundSubstitutionInteractionWithGroundTermMapping
 
   variable {sig : Signature} [DecidableEq sig.C] [DecidableEq sig.V]
 
-  theorem GroundSubstitution.apply_var_or_const_compose (s : GroundSubstitution sig) (h : GroundTermMapping sig) (id_on_const : h.isIdOnConstants) :
+  theorem GroundSubstitution.apply_var_or_const_compose (s : GroundSubstitution sig)
+      (h : GroundTermMapping sig) (id_on_const : h.isIdOnConstants) :
       ∀ (voc : VarOrConst sig), GroundSubstitution.apply_var_or_const (h ∘ s) voc = h (s.apply_var_or_const voc) := by
     intro voc
     unfold GroundSubstitution.apply_var_or_const
